getn back into swing of it

Cedille2/FomegaModel/Consistency.lean
@@ -1,19 +1,20 @@
 
-import WCCC.Proof
-import WCCC.Proof.Derivations
+import Cedille2.Proof
 import Fomega.Basic.Derivations
-import WCCC.FomegaModel.Interpretation
-import WCCC.FomegaModel.Normalization
+import Cedille2.FomegaModel.Interpretation
+import Cedille2.FomegaModel.Normalization
 
 namespace FomegaModel
 
-  theorem equational_consistency
-    : ¬ ([] ⊢c t : .eq cBool ctt cff)
-  := by sorry
+  def ctt : Cedille2.Term := λτ[★] λf[#!0] λf[#!1] #1
+  def cff : Cedille2.Term := λτ[★] λf[#!0] λf[#!1] #0
 
   theorem logical_consistency
     : ¬ ([] ⊢c t : cFalse)
   := by sorry
 
+  theorem equational_consistency
+    : ¬ ([] ⊢c t : .eq ctt cff)
+  := by sorry
 
 end FomegaModel
