Cedille2/FomegaModel/Normalization.lean
@@ -1,103 +1,31 @@
 
-import WCCC.Proof
+import Common
+import Cedille2.Proof
 import Fomega.Basic.Derivations
-import WCCC.FomegaModel.Interpretation
+import Cedille2.FomegaModel.Interpretation
 
 namespace FomegaModel
 
   theorem red_preserved :
     Γ ⊢c t : A ->
-    let ℓ := Γ.length
     t -β> s ->
-    ∃ z, 𝓉 ℓ t -β>+ z ∧ 𝓉 ℓ s -β>* z
+    𝓉 t -β>+ 𝓉 s
   := by
-  intro j ℓ r
-  induction r
-  case beta => sorry
-  case iproj1 =>
-    simp at *; sorry
-  case iproj2 => sorry
-  case proj1 => sorry
-  case proj2 => sorry
-  case substelim => sorry
-  case phi => sorry
-  case unit_rec => sorry
-  case conv_beta => sorry
-  case conv_fst => sorry
-  case conv_snd => sorry
-  case conv_subst => sorry
-  case conv_phi => sorry
-  case conv_conv =>
-    simp at *; sorry
-  case lam_congr1 => sorry
-  case lam_congr2 => sorry
-  case app_congr1 => sorry
-  case app_congr2 => sorry
-  case all_congr1 => sorry
-  case all_congr2 => sorry
-  case inter_congr1 => sorry
-  case inter_congr2 => sorry
-  case inter_congr3 => sorry
-  case pair_congr1 => sorry
-  case pair_congr2 => sorry
-  case fst_congr => sorry
-  case snd_congr => sorry
-  case inter_ty_congr1 => sorry
-  case inter_ty_congr2 => sorry
-  case times_congr1 => sorry
-  case times_congr2 => sorry
-  case refl_congr1 => sorry
-  case refl_congr2 => sorry
-  case subst_congr1 => sorry
-  case subst_congr2 => sorry
-  case phi_congr1 => sorry
-  case phi_congr2 => sorry
-  case phi_congr3 => sorry
-  case phi_congr4 => sorry
-  case eq_congr1 => sorry
-  case eq_congr2 => sorry
-  case eq_congr3 => sorry
-  case conv_congr1 => sorry
-  case conv_congr2 => sorry
-  case unit_rec_congr1 => sorry
-  case unit_rec_congr2 => sorry
+  intro j r; sorry
 
   theorem fomega_sn_implies_sn :
     Γ ⊢c t : A ->
-    let ℓ := Γ.length
-    z -β>* 𝓉 ℓ t ->
-    Term.SNPlus z ->
-    Term.SN t
+    @SNPlus _ Fomega.Red (𝓉 t) ->
+    @SN _ Cedille2.Red t
   := by
-  intro j ℓ r h
-  induction h generalizing t
-  case _ s h ih =>
-    constructor; intro y r2
-    have lem := red_preserved j r2
-    cases lem; case _ z lem =>
+  sorry
 
-      sorry
-  -- generalize sdef : 𝓉 ℓ t = s at *
-  -- induction h generalizing t
-  -- case _ s h ih =>
-  --   rw [<-sdef] at ih
-  --   constructor; intro t' r
-  --   have lem := red_preserved j r
-  --   cases lem; case _ z lem =>
+  axiom fomega_sn {Γ : Ctx Fomega.Term} {t A : Fomega.Term} : Γ ⊢ω t : A -> @SN _ Fomega.Red t
 
-  --     sorry
-    --
-    -- -- step here requires preservation (as expected)
-    -- apply ih (𝓉 ℓ t') lem sorry rfl
-
-  axiom fomega_sn {Γ : Ctx} {t A : Term} : Γ ⊢ω t : A -> Term.SN t
-
-  theorem sn_term : Γ ⊢c t : A -> Term.SN t := by
+  theorem sn_term : Γ ⊢c t : A -> @SN _ Cedille2.Red t := by
   intro j; apply fomega_sn_implies_sn j
-  let ℓ := Γ.length
-  have lem1 : (γ Γ) ⊢ω (𝓉 ℓ t) : (𝒯 ℓ A) := by sorry
+  have lem1 : (γ Γ) ⊢ω (𝓉 t) : (𝒯 A) := by sorry
   have lem2 := fomega_sn lem1
-  have lem3 : Γ.length = ℓ := by unfold ℓ; simp
-  rw [lem3]; apply Term.sn_implies_snplus; apply lem2
+  apply sn_implies_snplus; apply lem2
 
 end FomegaModel
