Cedille2/FomegaModel/Soundness.lean
@@ -1,0 +1,44 @@
+
+import Cedille2.Proof
+import Fomega.Basic.Derivations
+import Cedille2.FomegaModel.Interpretation
+import Cedille2.FomegaModel.Normalization
+
+namespace FomegaModel
+
+  @[simp]
+  abbrev KindSoundnessLemmaType : (v : Cedille2.JudgmentVariant) -> Cedille2.JudgmentIndex v -> Prop
+  | .prf => λ (t, A) => A = (□ : Cedille2.Term) -> ∀ Δ, ⊢ω Δ -> Δ ⊢ 𝒱 t : □
+  | .wf => λ _ => True
+
+  theorem kind_soundness_lemma : Cedille2.Judgment v Γ ix -> KindSoundnessLemmaType v ix := by
+  intro j
+  induction j <;> simp at *
+  case _ => sorry
+  case _ => sorry
+  case _ => sorry
+  case _ => sorry
+  case _ => sorry
+  case _ => sorry
+  case _ => sorry
+  case _ => sorry
+
+  theorem kind_soundness :
+    Γ ⊢c t : □ ->
+    ∀ Δ, ⊢ω Δ -> Δ ⊢ 𝒱 t : □
+  := by
+  intro j
+  apply kind_soundness_lemma j rfl
+
+  theorem type_soundness :
+    Γ ⊢c t : A ->
+    Γ ⊢c A : □ ->
+    γ Γ ⊢ 𝒯 t : 𝒱 A
+  := by sorry
+
+  theorem term_soundness :
+    Γ ⊢c t : A ->
+    γ Γ ⊢ 𝓉 t : 𝒯 A
+  := by sorry
+
+end FomegaModel
