Cedille2/Term/Erasure.lean
@@ -1,8 +1,10 @@
 import Common
 import Erased.Term
 import Cedille2.Term
+import Cedille2.Term.Classify
 
 namespace Cedille2.Term
+  @[simp]
   def erase : Term -> Erased.Term
   | .var K x => .var K x
   | .const K => .const K
@@ -11,7 +13,7 @@ namespace Cedille2.Term
   | .app m0 f _ => erase f
   | .lam mt A t => .lamt (erase A) (erase t)
   | .lam mf _ t => .lam (erase t)
-  | .lam m0 _ t => erase t
+  | .lam m0 _ t => erase (t β[□])
   | .all m A B => .all m (erase A) (erase B)
   | .inter _ _ _ t _ => erase t
   | .fst t => erase t
@@ -22,4 +24,212 @@ namespace Cedille2.Term
   | .subst _ _ t => erase t
   | .phi a _ _ => erase a
   | .conv _ _ _ t => erase t
+  termination_by t => Term.size t
+  decreasing_by
+    all_goals (simp; try omega)
+    rw [size_of_subst]; omega
+    intro n; unfold action_size
+    cases n <;> simp
 end Cedille2.Term
+
+namespace Erased.Term
+  @[simp]
+  def embed : Term -> Cedille2.Term
+  | var K x => .var K x
+  | const K => .const K
+  | appt f a => .app mt (embed f) (embed a)
+  | app f a => .app mf (embed f) (embed a)
+  | lamt A t => .lam mt (embed A) (embed t)
+  | lam t => .lam mf □ (embed t)
+  | all m A B => .all m (embed A) (embed B)
+  | inter_ty A B => .inter_ty (embed A) (embed B)
+  | eq a b => .eq (embed a) (embed b)
+end Erased.Term
+
+namespace Cedille2
+
+  theorem erase_rename_with_const_lemma {r : Ren} :
+    (∀ {n t}, σ n = .su t -> ∃ K, t = .const K) ->
+    Subst.map Term.erase (r.to ⊙ σ) = Subst.map Term.erase r.to ⊙ Subst.map Term.erase σ
+  := by
+  intro h
+  funext; case _ x =>
+    unfold Subst.compose; simp
+    generalize zdef : σ x = z at *
+    cases z <;> simp at *
+    case _ t =>
+      replace h := h zdef
+      cases h; case _ k h =>
+        subst h; simp
+
+  theorem subst_is_const_lift σ :
+    (∀ {n t}, σ n = .su t -> ∃ K, t = .const K) ->
+    (∀ {n t}, ^σ n = .su t -> ∃ K, t = Term.const K)
+  := by
+  intro h1 n t h2; simp at *
+  cases n <;> simp at *
+  case _ n =>
+    unfold Subst.compose at h2; simp at h2
+    generalize zdef : σ n = z at h2
+    cases z
+    case _ k => simp at h2
+    case _ t' =>
+      simp at h2
+      replace h1 := h1 zdef
+      cases h1; case _ K h1 =>
+        subst h2; subst h1; simp
+
+  theorem erase_rename_with_const :
+    (∀ {n t}, σ n = .su t -> ∃ K, t = .const K) ->
+    Term.erase ([σ]t) = [Subst.map Term.erase σ](Term.erase t)
+  := by
+  intro h
+  induction t generalizing σ <;> simp
+  case _ K x =>
+    generalize zdef : σ x = z at *
+    cases z <;> simp at *
+  case _ m f a ih1 ih2 =>
+    cases m <;> simp at *
+    case _ => rw [ih1 h, ih2 h]; simp
+    case _ => rw [ih1 h]
+    case _ => rw [ih1 h, ih2 h]; simp
+  case _ m A t ih1 ih2 =>
+    cases m
+    case _ =>
+      have lem1 := @ih2 (^σ) (subst_is_const_lift σ h); simp at *
+      rw [lem1, <-to_S, erase_rename_with_const_lemma h, to_S]
+      simp
+    case _ =>
+      have lem1 := @ih2 (.su □ :: I)
+      have lem2 := @ih2 (.su □ :: σ)
+      simp at *
+      rw [lem1, lem2]; simp
+      case _ =>
+        intro n t h2
+        cases n <;> simp at *
+        case _ => subst t; simp
+        case _ n => apply h h2
+      case _ =>
+        intro n t h2
+        cases n <;> simp at *
+        case _ => subst t; simp
+    case _ =>
+      have lem1 := @ih2 (^σ) (subst_is_const_lift σ h); simp at *
+      rw [lem1, <-to_S, erase_rename_with_const_lemma h, to_S]
+      simp; apply ih1 h
+  case _ ih1 ih2 =>
+    have lem1 := @ih2 (^σ) (subst_is_const_lift σ h); simp at *
+    rw [lem1, <-to_S, erase_rename_with_const_lemma h, to_S]
+    simp; apply ih1 h
+  case _ ih _ => apply ih h
+  case _ ih => apply ih h
+  case _ ih => apply ih h
+  case _ ih1 ih2 =>
+    have lem1 := @ih2 (^σ) (subst_is_const_lift σ h); simp at *
+    rw [lem1, <-to_S, erase_rename_with_const_lemma h, to_S]
+    simp; apply ih1 h
+  case _ ih1 ih2 => apply And.intro (ih1 h) (ih2 h)
+  case _ ih => apply ih h
+  case _ ih _ _ => apply ih h
+  case _ ih => apply ih h
+
+  theorem erase_rename_commute {r : Ren}
+    : ∀ t, Term.erase ([r.to]t) = [r.to](Term.erase t)
+  := by
+  intro t
+  induction t generalizing r <;> simp
+  case _ => unfold Ren.to; simp
+  case _ m f a ih1 ih2 =>
+    cases m <;> simp at *
+    case _ => rw [ih1, ih2]; simp
+    case _ => rw [ih1]
+    case _ => rw [ih1, ih2]; simp
+  case _ m A t ih1 ih2 =>
+    cases m <;> simp at *
+    case _ =>
+      have lem := @ih2 (Ren.lift r); rw [Subst.lift_lemma] at lem; simp at lem
+      rw [lem, Subst.lift_lemma]; simp
+    case _ =>
+      rw [erase_rename_with_const, erase_rename_with_const]; simp
+      case _ =>
+        intro n t h
+        cases n <;> simp at *
+        subst h; exists .kind
+      case _ =>
+        intro n t h
+        cases n <;> simp at *
+        case _ => subst h; exists .kind
+        case _ =>
+          unfold Ren.to at h; simp at h
+    case _ =>
+      rw [ih1]; apply And.intro rfl
+      have lem := @ih2 (Ren.lift r); rw [Subst.lift_lemma] at lem; simp at lem
+      rw [lem, Subst.lift_lemma]; simp
+  case _ ih1 ih2 =>
+    rw [ih1]; apply And.intro rfl
+    have lem := @ih2 (Ren.lift r); rw [Subst.lift_lemma] at lem; simp at lem
+    rw [lem, Subst.lift_lemma]; simp
+  case _ ih _ => apply ih
+  case _ ih => apply ih
+  case _ ih => apply ih
+  case _ ih1 ih2 =>
+    rw [ih1]; apply And.intro rfl
+    have lem := @ih2 (Ren.lift r); rw [Subst.lift_lemma] at lem; simp at lem
+    rw [lem, Subst.lift_lemma]; simp
+  case _ ih1 ih2 => apply And.intro ih1 ih2
+  case _ ih => apply ih
+  case _ ih _ _ => apply ih
+  case _ ih => apply ih
+
+  theorem erase_subst {t : Term} : ([σ]t).erase = [Subst.map Term.erase σ]t.erase := by
+  have lem : ∀ {T}, S = @Ren.to T (λ x => x + 1) := by
+    unfold S; unfold Ren.to; simp
+  induction t generalizing σ <;> simp
+  case _ K x =>
+    generalize zdef : σ x = z at *
+    cases z <;> simp at *
+  case _ m f a ih1 ih2 =>
+    cases m <;> simp
+    case _ =>
+      rw [ih1, ih2]; apply And.intro rfl rfl
+    case _ => apply ih1
+    case _ =>
+      rw [ih1, ih2]; apply And.intro rfl rfl
+  case _ m A t ih1 ih2 =>
+    cases m <;> simp
+    case _ =>
+      have lem2 := @ih2 (^σ); simp at lem2
+      rw [lem2, lem, lem, Subst.map_rename_compose_left erase_rename_commute]
+    case _ =>
+      rw [@erase_rename_with_const (.su □ :: I)]; simp
+      have lem2 := @ih2 (.su □ :: σ); simp at lem2
+      rw [lem2]
+      case _ =>
+        intro n t h
+        cases n <;> simp at *
+        subst h; exists .kind
+    case _ =>
+      have lem2 := @ih2 (^σ); simp at lem2
+      rw [lem2, lem, lem, Subst.map_rename_compose_left erase_rename_commute]
+      apply And.intro ih1; rfl
+  case _ ih1 ih2 =>
+    have lem2 := @ih2 (^σ); simp at lem2
+    rw [lem2, lem, lem, Subst.map_rename_compose_left erase_rename_commute]
+    apply And.intro ih1; rfl
+  case _ ih _ => apply ih
+  case _ ih => apply ih
+  case _ ih => apply ih
+  case _ ih1 ih2 =>
+    have lem2 := @ih2 (^σ); simp at lem2
+    rw [lem2, lem, lem, Subst.map_rename_compose_left erase_rename_commute]
+    apply And.intro ih1; rfl
+  case _ ih1 ih2 => apply And.intro ih1 ih2
+  case _ ih => apply ih
+  case _ ih _ _ => apply ih
+  case _ ih => apply ih
+
+  theorem erase_beta {b t : Term} : (b β[t]).erase = b.erase β[t.erase] := by
+  have lem := @erase_subst (.su t :: I) b; simp at lem
+  apply lem
+
+end Cedille2
